bump & fix

Algorithm/Data/Graph.lean
@@ -3,63 +3,46 @@ import Algorithm.Data.Classes.AssocArray
 import Algorithm.Data.Classes.Collection
 import Mathlib.Data.List.Nodup
 
-structure Graph where
-  V : Type*
-  [decidableEqV : DecidableEq V]
-  EType : Type*
-  [decidableEqEType : DecidableEq EType]
-  EColl : Type*
-  [collectionEColl : Collection EColl EType]
-  fst' : EType → V
-  snd' : EType → V
-  StarList : Type*
-  [inhabitedEColl : Inhabited EColl]
-  [assocArrayStarList : AssocArray StarList V EColl]
-  star' : StarList
-  costar' : StarList
-  fst_star' v : ∀ e ∈ star'[v], fst' e = v
-  snd_costar' v : ∀ e ∈ costar'[v], snd' e = v
-  count_star'_fst_eq_count_costar'_snd e :
-    Collection.count e star'[fst' e] = Collection.count e costar'[snd' e]
+structure Graph
+    (V : Type*) [DecidableEq V]
+    (EType : Type*) [DecidableEq EType]
+    (EColl : Type*) [Collection EColl EType] [Inhabited EColl]
+    (StarList : Type*) [AssocArray StarList V EColl] where
+  fst : EType → V
+  snd : EType → V
+  star : StarList
+  costar : StarList
+  fst_star v : ∀ e ∈ star[v], fst e = v
+  snd_costar v : ∀ e ∈ costar[v], snd e = v
+  count_star_fst_eq_count_costar_snd e :
+    Collection.count e star[fst e] = Collection.count e costar[snd e]
   -- nodup_star' (v : V) : star'[v].Nodup
   -- nodup_costar' (v : V) : costar'[v].Nodup
   -- mem_star'_iff_mem_costar' e : e ∈ star'[fst' e] ↔ e ∈ costar'[snd' e]
 
 namespace Graph
 
-attribute [instance] decidableEqV decidableEqEType collectionEColl inhabitedEColl
-  assocArrayStarList
-
-variable {g : Graph}
+variable
+  {V : Type*} [DecidableEq V]
+  {EType : Type*} [DecidableEq EType]
+  {EColl : Type*} [Collection EColl EType] [Inhabited EColl]
+  {StarList : Type*} [AssocArray StarList V EColl] {g : Graph V EType EColl StarList}
 -- instance : GetElem g.StarList g.V (List g.E) (fun _ _ ↦ True) := AssocArray.instGetElem
 -- by infer_instance
-
-def EType.fst (e : g.EType) : g.V := g.fst' e
-def EType.snd (e : g.EType) : g.V := g.snd' e
-
-def V.star (v : g.V) : g.EColl := g.star'[v]
-def V.costar (v : g.V) : g.EColl := g.costar'[v]
-
-lemma fst_star (v : g.V) : ∀ e ∈ v.star, e.fst = v := g.fst_star' v
-lemma snd_costar (v : g.V) : ∀ e ∈ v.costar, e.snd = v := g.snd_costar' v
-
-lemma count_star_fst_eq_count_costar_snd (e : g.EType) :
-    Collection.count e e.fst.star = Collection.count e e.snd.costar :=
-  g.count_star'_fst_eq_count_costar'_snd e
 
 -- lemma nodup_star (v : g.V) : v.star.Nodup := g.nodup_star' v
 -- lemma nodup_costar (v : g.V) : v.costar.Nodup := g.nodup_costar' v
 
-lemma mem_star_iff_mem_costar (e : g.EType) : e ∈ e.fst.star ↔ e ∈ e.snd.costar := by
+lemma mem_star_iff_mem_costar (e : EType) : e ∈ g.star[g.fst e] ↔ e ∈ g.costar[g.snd e] := by
   rw [← Collection.count_ne_zero, ← Collection.count_ne_zero,
     count_star_fst_eq_count_costar_snd]
 
-def E (g : Graph) := {e : g.EType // e ∈ e.fst.star}
+def E (g : Graph V EType EColl StarList) := {e : EType // e ∈ g.star[g.fst e]}
 
-def E.fst (e : g.E) : g.V := e.val.fst
-def E.snd (e : g.E) : g.V := e.val.snd
+def E.fst (e : g.E) : V := g.fst e.val
+def E.snd (e : g.E) : V := g.snd e.val
 
-lemma E.mem_star (e : g.E) : e.val ∈ e.fst.star := e.2
-lemma E.mem_costar (e : g.E) : e.val ∈ e.snd.costar := (mem_star_iff_mem_costar _).mp e.2
+lemma E.mem_star (e : g.E) : e.val ∈ g.star[e.fst] := e.2
+lemma E.mem_costar (e : g.E) : e.val ∈ g.costar[e.snd] := (mem_star_iff_mem_costar _).mp e.2
 
 end Graph
