lakefile.lean
@@ -1,14 +1,17 @@
 import Lake
 open Lake DSL
 
-package algorithm {
-  moreServerArgs := #["-DautoImplicit=false"]
-}
+package algorithm where
+  leanOptions := #[
+    ⟨`pp.unicode.fun, true⟩, -- pretty-prints `fun a ↦ b`
+    ⟨`pp.proofs.withType, false⟩,
+    ⟨`autoImplicit, false⟩,
+    ⟨`relaxedAutoImplicit, false⟩
+  ]
 
 require mathlib from git "https://github.com/leanprover-community/mathlib4.git" @ "master"
 
 @[default_target]
 lean_lib Algorithm {
   roots := #[`Algorithm]
-  moreLeanArgs := #["-DautoImplicit=false"]
 }
